code/bignum/Hacl.Bignum.fsti
@@ -338,29 +338,12 @@ class bn (t:limb_t) = {
   sqr: a:lbignum t len -> bn_karatsuba_sqr_st a;
 }
 
-let add_mod_n32: len:size_t{v len > 0} -> bn_add_mod_n_st U32 len
- = bn_add_mod_n #U32
 
-let add_mod_n64: len:size_t{v len > 0} -> bn_add_mod_n_st U64 len
- = bn_add_mod_n #U64
-
-// Prevent inlining
 inline_for_extraction noextract
-let add_mod_n' (#t:limb_t): len:size_t{v len > 0} -> bn_add_mod_n_st t len
- = match t with | U32 -> add_mod_n32 | U64 -> add_mod_n64
+val mk_runtime_bn: t:limb_t -> len:meta_len t -> bn t
 
-/// This is a default implementation that *will* generate code depending on
-/// `len` at run-time! Only use if you want to generate run-time generic
-/// functions!
-inline_for_extraction noextract
-let mk_runtime_bn (t:limb_t) (len:meta_len t) = {
-  len = len;
-  add = (fun a b -> bn_add_eq_len len a b);
-  sub = (fun a b -> bn_sub_eq_len len a b);
-  add_mod_n = add_mod_n' len;
-  mul = (fun a b -> bn_karatsuba_mul len a b);
-  sqr = (fun a -> bn_karatsuba_sqr len a);
-}
+val mk_runtime_bn_len_lemma: t:limb_t -> len:meta_len t ->
+  Lemma ((mk_runtime_bn t len).len == len) [SMTPat (mk_runtime_bn t len)]
 
 ///
 ///  Bignum comparison and test functions
