code/bignum/Hacl.Bignum.Montgomery.fsti
@@ -165,4 +165,4 @@ inline_for_extraction noextract
 val mk_runtime_mont: #t:limb_t -> len:BN.meta_len t -> mont t
 
 val mk_runtime_mont_len_lemma: #t:limb_t -> len:BN.meta_len t ->
-  Lemma ((mk_runtime_mont #t len).bn.BN.len == len)
+  Lemma ((mk_runtime_mont #t len).bn.BN.len == len) [SMTPat (mk_runtime_mont #t len)]
